Full caching example in TrivialCache.

examples/TrivialCache.v
@@ -1,5 +1,3 @@
-Ltac typeof' H := type of H.
-
 Require Import QueryStructureNotations.
 Require Import ListImplementation.
 Require Import AddCache ADTCache.
@@ -21,6 +19,7 @@ Definition Dog := TupleDef MySchema "Dog".
 Definition MySig : ADTSig :=
   ADTsignature {
       "Empty" : unit → rep,
+      "AddDog" : rep × Dog → rep × unit,
       "YoungOwners'Breeds" : rep × nat → rep × list string,
       "BreedPopulation" : rep × string → rep × nat
   }.
@@ -28,6 +27,9 @@ Definition MySig : ADTSig :=
 Definition MySpec : ADT MySig :=
   QueryADTRep MySchema {
     const "Empty" (_ : unit) : rep := empty,
+
+   update "AddDog" (dog : Dog) : unit :=
+      Insert dog into "Dog",
 
     query "YoungOwners'Breeds" ( ageLimit : nat ) : list string :=
       For (d in "Dog")
@@ -42,19 +44,19 @@ Definition MySpec : ADT MySig :=
                    Return ())
 }.
 
-Definition BreedCacheSpec (or : UnConstrQueryStructure MySchema)
-           (cache : string -> nat) :=
-forall breed,
-  refine
+Definition BreedCacheSpec (breed : string)
+           (or : UnConstrQueryStructure MySchema)
+           (cache : nat) :=
+    refine
     (Count (For (UnConstrQuery_In or ``("Dog")
                                   (fun d =>
                                      Where (d!"Breed" = breed)
-             Return ()))))
-    (ret (cache breed)).
+                                           Return ()))))
+    (ret cache).
 
 Definition MyListImpl_abs
-           (or : cachedRep (UnConstrQueryStructure MySchema) (string -> nat))
-           (nr : (list Person * list Dog) * (string -> nat)) : Prop :=
+           (or : cachedRep (UnConstrQueryStructure MySchema) nat)
+           (nr : (list Person * list Dog) * nat) : Prop :=
   ((origRep or) ! "Person" ≃ fst (fst nr) /\
   (origRep or) ! "Dog" ≃ snd (fst nr)) /\
   cachedVal or = snd nr.
@@ -66,7 +68,7 @@ Proof.
 
   start honing QueryStructure.
 
-  hone representation using (cachedRep_AbsR BreedCacheSpec).
+  hone representation using (cachedRep_AbsR (BreedCacheSpec "Dachshund")).
 
   hone method "YoungOwners'Breeds".
   { simplify with monad laws.
@@ -81,22 +83,106 @@ Proof.
     setoid_rewrite (refine_pick_val _ H0).
     simplify with monad laws; simpl.
     unfold cachedRep_AbsR in H0; intuition; subst.
-    unfold BreedCacheSpec in H2.
-    subst_body.
-    setoid_rewrite (H2 n); simplify with monad laws; simpl.
-    finish honing.
+    eapply refine_if with (b := if (string_dec n "Dachshund") 
+                                then true
+                                else false).
+    { find_if_inside; try congruence; subst.
+      intros; unfold BreedCacheSpec in H2.
+      subst_body.
+      setoid_rewrite H2; simplify with monad laws; simpl.
+      reflexivity. }
+    { find_if_inside; try congruence; subst.
+      simpl; reflexivity. 
+    }
   }
 
   hone constructor "Empty".
   { simplify with monad laws.
     rewrite refine_pick_cachedRep.
-    rewrite refine_pick_val with (A := string -> nat)
-                                   (a := fun x : string => 0).
+    rewrite refine_pick_val with (A := nat)
+                                   (a := 0).
     simplify with monad laws; finish honing.
     unfold BreedCacheSpec; simpl.
-    intros; setoid_rewrite refine_Count.
+    unfold pointwise_relation; intros; setoid_rewrite refine_Count.
     setoid_rewrite refine_For_In_Empty.
     simplify with monad laws; reflexivity.
+  }
+
+  Lemma refine_Where {A B} :
+    forall (P : Ensemble A)
+           (P_dec : DecideableEnsemble P)
+           (bod : Comp (list B)),
+      forall a,
+        refine (Where (P a) bod)
+               (if (dec a) then
+                  bod
+                else
+                  (ret [])).
+  Proof.
+    unfold refine, Query_Where; intros.
+    caseEq (dec a); rewrite H0 in H; econstructor;
+    split; intros; eauto.
+    apply dec_decides_P in H0; intuition.
+    apply Decides_false in H0; intuition.
+    inversion_by computes_to_inv; eauto.
+  Qed.
+
+  Lemma refine_Count_if {A} :
+    forall (b : bool) (t : A),
+      refine (Count (if b then Return t else ret []))
+             (ret (if b then 1 else 0)).
+  Proof.
+    intros; rewrite refine_Count.
+    destruct b; simplify with monad laws; reflexivity.
+  Qed.
+
+  hone method "AddDog".
+  {
+    simplify with monad laws; cbv beta; simpl.
+    etransitivity.
+    eapply refine_bind_pick; intros.
+    rewrite refine_pick_cachedRep.
+    simplify with monad laws.
+    unfold BreedCacheSpec; simpl.
+    pose_string_ids.
+
+    rewrite refine_pick_val.
+    simplify with monad laws; higher_order_1_reflexivity.
+    unfold pointwise_relation; intros.
+    intros; etransitivity.
+    apply refine_refine_Count.
+    apply refine_For_In_Insert.
+    unfold In, not; intros; eapply H1;
+    [ eapply H2
+     | subst_body; auto ].
+    rewrite refine_Count_bind_bind_app.
+    unfold cachedRep_AbsR, BreedCacheSpec in H0; split_and; subst.
+    pose_string_ids.
+    setoid_rewrite H3.
+    simplify with monad laws.
+    subst_body.
+    etransitivity.
+    pose (n!"Breed"); simpl in *.
+    eapply refine_if with (b := if (string_dec d "Dachshund") 
+                                then true
+                                else false);
+    find_if_inside; try congruence; intros.
+    subst_body.
+    rewrite refine_Count; simplify with monad laws.
+    unfold Query_Where, Query_Return.
+    rewrite refine_pick_val.
+    simplify with monad laws; reflexivity.
+    intuition.
+    rewrite refine_Count; simplify with monad laws.
+    unfold Query_Where, Query_Return.
+    rewrite refine_pick_val.
+    simplify with monad laws; reflexivity.
+    intuition.
+    eapply refineEquiv_if_ret.
+    simpl.
+    unfold cachedRep_AbsR in H0; intuition.
+    subst.
+    finish honing.
   }
 
   hone representation using MyListImpl_abs.
@@ -106,10 +192,10 @@ Proof.
     rewrite (@refineEquiv_pick_pair_pair
                   (list Person)
                   (list Dog)
-                  (string -> nat)
+                  (nat)
                   (EnsembleIndexedListEquivalence (fun _ : IndexedTuple => False))
                   (EnsembleIndexedListEquivalence (fun _ : IndexedTuple => False))
-                  (fun c : string -> nat => (fun _ => 0) = c)).
+                  (fun c : nat => 0 = c)).
     rewrite refine_pick_val by
         apply EnsembleIndexedListEquivalence_Empty;
     simplify with monad laws.
@@ -135,9 +221,10 @@ Proof.
     setoid_rewrite refineEquiv_pick_pair_pair.
     setoid_rewrite refineEquiv_pick_eq'.
     simplify with monad laws.
-    rewrite refine_pick_val by apply H0.
+    simpl in *.
+    rewrite refine_pick_val by eassumption.
     simplify with monad laws.
-    rewrite refine_pick_val by apply H3.
+    rewrite refine_pick_val by eassumption.
     simplify with monad laws.
     rewrite H2.
     finish honing.
@@ -145,19 +232,86 @@ Proof.
 
   hone method "BreedPopulation".
   {
+    eapply refine_if with (b := if (string_dec n "Dachshund") 
+                                then true
+                                else false);
+    find_if_inside; try congruence; intros;
     simplify with monad laws; simpl.
-    
-    unfold MyListImpl_abs in *; intuition.
-    setoid_rewrite refineEquiv_pick_pair_pair.
+
+    { 
+      unfold MyListImpl_abs in *; intuition.
+      setoid_rewrite refineEquiv_pick_pair_pair.
+      setoid_rewrite refineEquiv_pick_eq'.
+      simplify with monad laws.
+      rewrite refine_pick_val by eassumption.
+      simplify with monad laws.
+      rewrite refine_pick_val by eassumption.
+      simplify with monad laws.
+      rewrite H3.
+      reflexivity.
+    }
+
+    {
+      unfold MyListImpl_abs in *; split_and.
+      rewrite refine_Count; simplify with monad laws.
+      rewrite refine_List_Query_In by eassumption.
+      simpl; subst_body.
+      setoid_rewrite refine_List_Query_In_Where.
+      rewrite refine_List_For_Query_In_Return;
+        simplify with monad laws; simpl.
+      setoid_rewrite refineEquiv_pick_pair_pair.
+      setoid_rewrite refineEquiv_pick_eq'.
+      simplify with monad laws.
+      rewrite refine_pick_val by eassumption.
+      simplify with monad laws.
+      rewrite refine_pick_val by eassumption.
+      simplify with monad laws.
+      rewrite H3.
+      reflexivity.
+    }
+    }
+
+  hone method "AddDog".
+  {
+    unfold MyListImpl_abs in *; split_and.
+    simplify with monad laws; simpl.
+    rewrite refine_pick_val with (A := nat) (a := length (snd (fst r_n))).
+    simplify with monad laws; simpl.
+    pose_string_ids.
+    setoid_rewrite refineEquiv_pick_pair_pair; simpl.
     setoid_rewrite refineEquiv_pick_eq'.
     simplify with monad laws.
-    rewrite refine_pick_val by apply H0.
-    simplify with monad laws.
-    rewrite refine_pick_val by apply H3.
-    simplify with monad laws.
-    rewrite H2.
-    finish honing.
+    subst_strings. 
+      match goal with
+          |- context
+               [{a | EnsembleIndexedListEquivalence
+                       ((@UpdateUnConstrRelation ?QSSchema ?c ?Ridx
+                                                (EnsembleInsert ?n (?c!?R)))!?R')%QueryImpl a}%comp] =>
+          let H := fresh in
+          generalize ((@ImplementListInsert_neq QSSchema
+                                                {| bindex := R' |}
+                                                {| bindex := R |} n c)) as H; intros; setoid_rewrite H
+      end; try reflexivity; try eassumption.
+      simplify with monad laws.
+      match goal with
+          |- context
+               [{a | EnsembleIndexedListEquivalence
+                       ((@UpdateUnConstrRelation ?QSSchema ?c ?Ridx
+                                                (EnsembleInsert ?n (?c!?R)))!?R)%QueryImpl a}%comp] =>
+          let H := fresh in
+          generalize ((@ImplementListInsert_eq QSSchema
+                                                {| bindex := R |}
+                                                n c)) as H; intros; setoid_rewrite H
+      end; try reflexivity; try eassumption.
+      simplify with monad laws.
+      rewrite H2.
+      finish honing.
+      congruence.
+      intros; destruct H3 as [H3 _].
+      intros; eapply lt_irrefl.
+      setoid_rewrite <- H4 in H3; eapply H3.
+      eauto.
   }
-
+  
   finish sharpening.
 Defined.
